LogicalRefinement/Untyped/Basic.lean
@@ -55,75 +55,75 @@ inductive UntypedKind: List Nat -> Type
   | let_wit: UntypedKind [2]
   | refl: UntypedKind [0]
 
-inductive RawUntyped: Type
+inductive Untyped: Type
   | var (v: Nat)
 
   | const (c: UntypedKind [])
-  | unary (k: UntypedKind [0]) (t: RawUntyped)
+  | unary (k: UntypedKind [0]) (t: Untyped)
   -- TODO: let n?
-  | let_bin (k: UntypedKind [2]) (e: RawUntyped)
+  | let_bin (k: UntypedKind [2]) (e: Untyped)
   -- TODO: bin n? Can't, due to, of course, lack of nested inductive types...
-  | bin (k: UntypedKind [0, 0]) (l: RawUntyped) (r: RawUntyped)
+  | bin (k: UntypedKind [0, 0]) (l: Untyped) (r: Untyped)
   -- TODO: abs n?
-  | abs (k: UntypedKind [0, 1]) (A: RawUntyped) (t: RawUntyped)
-  | tri (k: UntypedKind [0, 0, 0]) (A: RawUntyped) (l: RawUntyped) (r: RawUntyped)
+  | abs (k: UntypedKind [0, 1]) (A: Untyped) (t: Untyped)
+  | tri (k: UntypedKind [0, 0, 0]) (A: Untyped) (l: Untyped) (r: Untyped)
   -- TODO: no cases?
-  | cases (k: UntypedKind [1, 0, 0, 0]) (K: RawUntyped) (d: RawUntyped) (l: RawUntyped) (r: RawUntyped)
+  | cases (k: UntypedKind [1, 0, 0, 0]) (K: Untyped) (d: Untyped) (l: Untyped) (r: Untyped)
 
 -- Types
-def RawUntyped.nats := const UntypedKind.nats
-def RawUntyped.pi := abs UntypedKind.pi
-def RawUntyped.sigma := abs UntypedKind.sigma
-def RawUntyped.coprod := bin UntypedKind.coprod
-def RawUntyped.set := abs UntypedKind.set
-def RawUntyped.assume := bin UntypedKind.assume
-def RawUntyped.intersect := abs UntypedKind.intersect
-def RawUntyped.union := abs UntypedKind.union
+def Untyped.nats := const UntypedKind.nats
+def Untyped.pi := abs UntypedKind.pi
+def Untyped.sigma := abs UntypedKind.sigma
+def Untyped.coprod := bin UntypedKind.coprod
+def Untyped.set := abs UntypedKind.set
+def Untyped.assume := bin UntypedKind.assume
+def Untyped.intersect := abs UntypedKind.intersect
+def Untyped.union := abs UntypedKind.union
 
 -- Propositions
-def RawUntyped.top := const UntypedKind.top
-def RawUntyped.bot := const UntypedKind.bot
-def RawUntyped.and := bin UntypedKind.and
-def RawUntyped.or := bin UntypedKind.or
-def RawUntyped.implies := bin UntypedKind.implies
-def RawUntyped.forall_ := abs UntypedKind.forall_
-def RawUntyped.exists_ := abs UntypedKind.exists_
-def RawUntyped.eq := tri UntypedKind.eq
+def Untyped.top := const UntypedKind.top
+def Untyped.bot := const UntypedKind.bot
+def Untyped.and := bin UntypedKind.and
+def Untyped.or := bin UntypedKind.or
+def Untyped.implies := bin UntypedKind.implies
+def Untyped.forall_ := abs UntypedKind.forall_
+def Untyped.exists_ := abs UntypedKind.exists_
+def Untyped.eq := tri UntypedKind.eq
 
 -- Terms
-def RawUntyped.zero := const UntypedKind.zero
-def RawUntyped.succ := const UntypedKind.succ
-def RawUntyped.lam := abs UntypedKind.lam
-def RawUntyped.app := bin UntypedKind.app
-def RawUntyped.pair := bin UntypedKind.pair
-def RawUntyped.proj := λb => unary (UntypedKind.proj b)
-def RawUntyped.inj := λb => unary (UntypedKind.inj b)
-def RawUntyped.case := cases UntypedKind.case
-def RawUntyped.elem := bin UntypedKind.elem
-def RawUntyped.let_set := let_bin UntypedKind.let_set
-def RawUntyped.lam_pr := abs UntypedKind.lam_pr
-def RawUntyped.app_pr := bin UntypedKind.app_pr
-def RawUntyped.lam_irrel := abs UntypedKind.lam_irrel
-def RawUntyped.app_irrel := bin UntypedKind.app_irrel
-def RawUntyped.repr := bin UntypedKind.repr
-def RawUntyped.let_repr := let_bin UntypedKind.let_repr
+def Untyped.zero := const UntypedKind.zero
+def Untyped.succ := const UntypedKind.succ
+def Untyped.lam := abs UntypedKind.lam
+def Untyped.app := bin UntypedKind.app
+def Untyped.pair := bin UntypedKind.pair
+def Untyped.proj := λb => unary (UntypedKind.proj b)
+def Untyped.inj := λb => unary (UntypedKind.inj b)
+def Untyped.case := cases UntypedKind.case
+def Untyped.elem := bin UntypedKind.elem
+def Untyped.let_set := let_bin UntypedKind.let_set
+def Untyped.lam_pr := abs UntypedKind.lam_pr
+def Untyped.app_pr := bin UntypedKind.app_pr
+def Untyped.lam_irrel := abs UntypedKind.lam_irrel
+def Untyped.app_irrel := bin UntypedKind.app_irrel
+def Untyped.repr := bin UntypedKind.repr
+def Untyped.let_repr := let_bin UntypedKind.let_repr
 
 -- Proofs
-def RawUntyped.nil := const UntypedKind.nil
-def RawUntyped.abort := unary UntypedKind.abort
-def RawUntyped.conj := bin UntypedKind.conj
-def RawUntyped.comp := λb => unary (UntypedKind.comp b)
-def RawUntyped.disj := λb => unary (UntypedKind.disj b)
-def RawUntyped.case_pr := cases UntypedKind.case_pr
-def RawUntyped.imp := bin UntypedKind.imp
-def RawUntyped.mp := bin UntypedKind.mp
-def RawUntyped.general := abs UntypedKind.general
-def RawUntyped.inst := bin UntypedKind.inst
-def RawUntyped.witness := bin UntypedKind.witness
-def RawUntyped.let_wit := let_bin UntypedKind.let_wit
-def RawUntyped.refl := unary UntypedKind.refl
+def Untyped.nil := const UntypedKind.nil
+def Untyped.abort := unary UntypedKind.abort
+def Untyped.conj := bin UntypedKind.conj
+def Untyped.comp := λb => unary (UntypedKind.comp b)
+def Untyped.disj := λb => unary (UntypedKind.disj b)
+def Untyped.case_pr := cases UntypedKind.case_pr
+def Untyped.imp := bin UntypedKind.imp
+def Untyped.mp := bin UntypedKind.mp
+def Untyped.general := abs UntypedKind.general
+def Untyped.inst := bin UntypedKind.inst
+def Untyped.witness := bin UntypedKind.witness
+def Untyped.let_wit := let_bin UntypedKind.let_wit
+def Untyped.refl := unary UntypedKind.refl
 
-@[simp] def RawUntyped.fv: RawUntyped -> Nat
+@[simp] def Untyped.fv: Untyped -> Nat
   | var v => Nat.succ v
   | const c => 0
   | unary _ t => fv t
@@ -133,7 +133,7 @@ def RawUntyped.refl := unary UntypedKind.refl
   | tri _ A l r => Nat.max (fv A) (Nat.max (fv l) (fv r))
   | cases _ K d l r => Nat.max (fv K - 1) (Nat.max (fv d) (Nat.max (fv l) (fv r)))
 
-@[simp] def RawUntyped.has_dep: RawUntyped -> Nat -> Prop
+@[simp] def Untyped.has_dep: Untyped -> Nat -> Prop
   | var v, i => v = i
   | const c, _ => False
   | unary _ t, i => has_dep t i
@@ -143,7 +143,7 @@ def RawUntyped.refl := unary UntypedKind.refl
   | tri _ A l r, i => has_dep A i ∨ has_dep l i ∨ has_dep r i
   | cases _ K d l r, i => has_dep K (i + 1) ∨ has_dep d i ∨ has_dep l i ∨ has_dep r i
 
-theorem RawUntyped.has_dep_implies_fv (u: RawUntyped): {i: Nat} ->
+theorem Untyped.has_dep_implies_fv (u: Untyped): {i: Nat} ->
   has_dep u i -> i < fv u := by {
     induction u with
     | var v =>
@@ -197,145 +197,3 @@ theorem RawUntyped.has_dep_implies_fv (u: RawUntyped): {i: Nat} ->
         | Or.inr (Or.inr H) => Or.inr (Or.inr (Ir H))
       )
   }
-
-structure Untyped (n: Nat) := (val: RawUntyped) (p: RawUntyped.fv val ≤ n)
-
-def Untyped.raw (val: RawUntyped): Untyped (RawUntyped.fv val) :=
-  Untyped.mk val (Nat.le_of_eq rfl)
-
-def Untyped.fv: Untyped n -> Fin (n + 1) 
-  | Untyped.mk val p => Fin.mk (RawUntyped.fv val) (Nat.le_lt_succ p)
-
--- Constructors
-def Untyped.var (v: Nat): Untyped (Nat.succ v) :=
-  Untyped.mk (RawUntyped.var v) (Nat.lt_succ_self _)
-def Untyped.const (c: UntypedKind []): Untyped n :=
-  Untyped.mk (RawUntyped.const c) (Nat.zero_le _)
-def Untyped.unary (c: UntypedKind [0]): Untyped n -> Untyped n
-  | u => Untyped.mk (RawUntyped.unary c u.val) u.p
-def Untyped.let_bin (c: UntypedKind [2]): Untyped (n + 2) -> Untyped n
-  | u => Untyped.mk (RawUntyped.let_bin c u.val) (by {
-    simp only [RawUntyped.fv, Nat.le_sub_is_le_add]
-    exact u.p
-  })
-def Untyped.bin (c: UntypedKind [0, 0]): 
-  Untyped n -> Untyped n -> Untyped n
-  | l, r => Untyped.mk (RawUntyped.bin c l.val r.val) (by {
-    simp only [RawUntyped.fv, Nat.max_r_le_split]
-    exact ⟨l.p, r.p⟩
-  })
-def Untyped.abs (c: UntypedKind [0, 1]): 
-  Untyped n -> Untyped (n + 1) -> Untyped n
-  | l, r => Untyped.mk (RawUntyped.abs c l.val r.val) (by {
-    simp only [RawUntyped.fv, Nat.max_r_le_split]
-    apply And.intro;
-    case left => exact l.p
-    case right => 
-      simp only [RawUntyped.fv, Nat.le_sub_is_le_add]
-      exact r.p
-  })
-def Untyped.tri (c: UntypedKind [0, 0, 0]): 
-  Untyped n -> Untyped n -> Untyped n -> Untyped n
-  | A, l, r => Untyped.mk (RawUntyped.tri c A.val l.val r.val) (by {
-    simp only [RawUntyped.fv, Nat.max_r_le_split]
-    exact ⟨A.p, l.p, r.p⟩
-  })
-def Untyped.cases (c: UntypedKind [1, 0, 0, 0]):
-  Untyped (n + 1) -> Untyped n -> Untyped n -> Untyped n -> Untyped n
-  | K, d, l, r =>
-    Untyped.mk (RawUntyped.cases c K.val d.val l.val r.val) (by {
-      simp only [RawUntyped.fv, Nat.max_r_le_split]
-      apply And.intro;
-      case left => simp only [Nat.le_sub_is_le_add]; apply K.p
-      case right => exact ⟨d.p, l.p, r.p⟩
-    })
-
--- Types
-def Untyped.nats: Untyped n := const UntypedKind.nats
-def Untyped.pi: Untyped n -> Untyped (n + 1) -> Untyped n := 
-  abs UntypedKind.pi
-def Untyped.sigma: Untyped n -> Untyped (n + 1) -> Untyped n := 
-  abs UntypedKind.sigma
-def Untyped.coprod: Untyped n -> Untyped n -> Untyped n 
-  := bin UntypedKind.coprod
-def Untyped.set: Untyped n -> Untyped (n + 1) -> Untyped n 
-  := abs UntypedKind.set
-def Untyped.assume: Untyped n -> Untyped n -> Untyped n 
-  := bin UntypedKind.assume
-def Untyped.intersect: Untyped n -> Untyped (n + 1) -> Untyped n 
-  := abs UntypedKind.intersect
-def Untyped.union: Untyped n -> Untyped (n + 1) -> Untyped n 
-  := abs UntypedKind.union
-
--- Propositions
-def Untyped.top: Untyped n := const UntypedKind.top
-def Untyped.bot: Untyped n := const UntypedKind.bot
-def Untyped.and: Untyped n -> Untyped n -> Untyped n 
-  := bin UntypedKind.and
-def Untyped.or: Untyped n -> Untyped n -> Untyped n 
-  := bin UntypedKind.or
-def Untyped.implies: Untyped n -> Untyped n -> Untyped n 
-  := bin UntypedKind.implies
-def Untyped.forall_: Untyped n -> Untyped (n + 1) -> Untyped n
-  := abs UntypedKind.forall_
-def Untyped.exists_: Untyped n -> Untyped (n + 1) -> Untyped n 
-  := abs UntypedKind.exists_
-def Untyped.eq: Untyped n -> Untyped n -> Untyped n -> Untyped n
-  := tri UntypedKind.eq
-
--- Terms
-def Untyped.zero: Untyped n := const (UntypedKind.zero)
-def Untyped.succ: Untyped n := const (UntypedKind.succ)
-def Untyped.lam: Untyped n -> Untyped (n + 1) -> Untyped n
-   := abs UntypedKind.lam
-def Untyped.app: Untyped n -> Untyped n -> Untyped n 
-  := bin UntypedKind.app
-def Untyped.pair: Untyped n -> Untyped n -> Untyped n 
-  := bin UntypedKind.pair
-def Untyped.proj (b: Bool): Untyped n -> Untyped n 
-  := unary (UntypedKind.proj b)
-def Untyped.inj (b: Bool): Untyped n -> Untyped n 
-  := unary (UntypedKind.inj b)
-def Untyped.case: Untyped (n + 1) -> Untyped n -> Untyped n -> Untyped n -> Untyped n 
-  := cases UntypedKind.case
-def Untyped.elem: Untyped n -> Untyped n -> Untyped n 
-  := bin UntypedKind.elem
-def Untyped.let_set: Untyped (n + 2) -> Untyped n := 
-  let_bin UntypedKind.let_set
-def Untyped.lam_pr: Untyped n -> Untyped (n + 1) -> Untyped n
-  := abs UntypedKind.lam_pr
-def Untyped.app_pr: Untyped n -> Untyped n -> Untyped n 
-  := bin UntypedKind.app_pr
-def Untyped.lam_irrel: Untyped n -> Untyped (n + 1) -> Untyped n
-  := abs UntypedKind.lam_irrel
-def Untyped.app_irrel: Untyped n -> Untyped n -> Untyped n
-  := bin UntypedKind.app_irrel
-def Untyped.repr: Untyped n -> Untyped n -> Untyped n 
-  := bin UntypedKind.repr
-def Untyped.let_repr: Untyped (n + 2) -> Untyped n
-  := let_bin UntypedKind.let_repr
-
--- Proofs
-def Untyped.nil: Untyped n := const UntypedKind.nil
-def Untyped.abort: Untyped n -> Untyped n := unary UntypedKind.abort
-def Untyped.conj: Untyped n -> Untyped n -> Untyped n 
-  := bin UntypedKind.conj
-def Untyped.comp (b: Bool): Untyped n -> Untyped n 
-  := unary (UntypedKind.comp b)
-def Untyped.disj (b: Bool): Untyped n -> Untyped n 
-  := unary (UntypedKind.disj b)
-def Untyped.case_pr: Untyped (n + 1) -> Untyped n -> Untyped n -> Untyped n -> Untyped n 
-  := cases UntypedKind.case_pr
-def Untyped.imp: Untyped n -> Untyped n -> Untyped n 
-  := bin UntypedKind.imp
-def Untyped.mp: Untyped n -> Untyped n -> Untyped n 
-  := bin UntypedKind.mp
-def Untyped.general: Untyped n -> Untyped (n + 1) -> Untyped n
-  := abs UntypedKind.general
-def Untyped.inst: Untyped n -> Untyped n -> Untyped n 
-  := bin UntypedKind.inst
-def Untyped.witness: Untyped n -> Untyped n -> Untyped n 
-  := bin UntypedKind.witness
-def Untyped.let_wit: Untyped (n + 2) -> Untyped n
-  := let_bin UntypedKind.let_wit
-def Untyped.refl: Untyped n -> Untyped n := unary UntypedKind.refl
