LogicalRefinement/Untyped/Wk.lean
@@ -2,8 +2,8 @@ import LogicalRefinement.Utils
 import LogicalRefinement.Wk
 import LogicalRefinement.Untyped.Basic
 
-@[simp] def RawUntyped.wk: RawUntyped -> RawWk -> RawUntyped
-  | var v, ρ => var (RawWk.var ρ v)
+@[simp] def Untyped.wk: Untyped -> Wk -> Untyped
+  | var v, ρ => var (Wk.var ρ v)
   | const c, ρ => const c
   | unary k t, ρ => unary k (t.wk ρ)
   | let_bin k e, ρ => let_bin k (e.wk (ρ.liftn 2))
@@ -12,23 +12,23 @@ import LogicalRefinement.Untyped.Basic
   | tri k A l r, ρ => tri k (A.wk ρ) (l.wk ρ) (r.wk ρ)
   | cases k K d l r, ρ => cases k (K.wk ρ.lift) (d.wk ρ) (l.wk ρ) (r.wk ρ)
 
-@[simp] def RawUntyped.wk1 (u: RawUntyped) 
-  := u.wk RawWk.wk1
+@[simp] def Untyped.wk1 (u: Untyped) 
+  := u.wk Wk.wk1
 
-def RawUntyped.wk1_def {u: RawUntyped}: u.wk1 = u.wk RawWk.wk1 := rfl
+def Untyped.wk1_def {u: Untyped}: u.wk1 = u.wk Wk.wk1 := rfl
 
-@[simp] def RawUntyped.lift1 (u: RawUntyped) := u.wk (RawWk.lift RawWk.id)
+@[simp] def Untyped.lift1 (u: Untyped) := u.wk (Wk.lift Wk.id)
 
-@[simp] def RawUntyped.wkn (u: RawUntyped) (n: Nat) 
-  := u.wk (RawWk.wkn n)
+@[simp] def Untyped.wkn (u: Untyped) (n: Nat) 
+  := u.wk (Wk.wkn n)
 
-@[simp] def RawUntyped.wknth (u: RawUntyped) (n: Nat) 
-  := u.wk (RawWk.wknth n)
+@[simp] def Untyped.wknth (u: Untyped) (n: Nat) 
+  := u.wk (Wk.wknth n)
 
-def RawUntyped.wknth_def {u: RawUntyped} {n}: u.wknth n = u.wk (RawWk.wknth n) := rfl
+def Untyped.wknth_def {u: Untyped} {n}: u.wknth n = u.wk (Wk.wknth n) := rfl
 
-@[simp] def RawUntyped.wk_coherent: {u: RawUntyped} -> {ρ σ: RawWk} ->
-  RawWk.equiv ρ σ -> u.wk ρ = u.wk σ := by {
+@[simp] def Untyped.wk_coherent: {u: Untyped} -> {ρ σ: Wk} ->
+  Wk.equiv ρ σ -> u.wk ρ = u.wk σ := by {
   intro u;
   induction u with
   | var v => intros ρ σ H; simp only [wk]; rw [H]
@@ -37,29 +37,29 @@ def RawUntyped.wknth_def {u: RawUntyped} {n}: u.wknth n = u.wk (RawWk.wknth n) :
   | let_bin k e I => 
     intros ρ σ H;
     simp only [wk];
-    simp only [I (@RawWk.liftn_equiv 2 _ _ H)]
+    simp only [I (@Wk.liftn_equiv 2 _ _ H)]
   | bin k l r Il Ir => intros ρ σ H; simp [Il H, Ir H]
   | abs k A s IHA IHs =>
     intros ρ σ H;
     simp only [wk];
-    simp only [IHA H, IHs (RawWk.lift_equiv H)]
+    simp only [IHA H, IHs (Wk.lift_equiv H)]
   | tri k A l r IA Il Ir => intros ρ σ H; simp [IA H, Il H, Ir H]
   | cases k K d l r IK Id Il Ir => 
     intros ρ σ H; 
     simp only [wk];
-    simp [IK (RawWk.lift_equiv H), Id H, Il H, Ir H]
+    simp [IK (Wk.lift_equiv H), Id H, Il H, Ir H]
 }
 
-@[simp] def RawUntyped.wk_id {u: RawUntyped}: u.wk (RawWk.id) = u := by {
+@[simp] def Untyped.wk_id {u: Untyped}: u.wk (Wk.id) = u := by {
   induction u;
   case var => simp
   repeat simp only [
-    wk, RawUntyped.wk_coherent (RawWk.liftn_id_equiv), 
-    RawUntyped.wk_coherent RawWk.lift_id_equiv,
+    wk, Untyped.wk_coherent (Wk.liftn_id_equiv), 
+    Untyped.wk_coherent Wk.lift_id_equiv,
   *]
 }
 
-def RawUntyped.wk_bounds {u: RawUntyped}: {n m: Nat} -> {ρ: RawWk} ->
+def Untyped.wk_bounds {u: Untyped}: {n m: Nat} -> {ρ: Wk} ->
   wk_maps n m ρ -> fv u ≤ m -> fv (u.wk ρ) ≤ n := by {
     induction u with
     | var v => intros _ _ ρ Hm. apply Hm
@@ -114,24 +114,18 @@ def RawUntyped.wk_bounds {u: RawUntyped}: {n m: Nat} -> {ρ: RawWk} ->
           case right => apply IHr Hm Hr
   }
 
-def RawUntyped.fv_wk1: fv (wk1 u) ≤ fv u + 1 
+def Untyped.fv_wk1: fv (wk1 u) ≤ fv u + 1 
   := by apply wk_bounds wk_maps_wk1; exact Nat.le_refl _
 
-@[simp] def RawUntyped.wk_composes {u: RawUntyped}: 
-  (σ ρ: RawWk) -> (u.wk ρ).wk σ = u.wk (σ.comp ρ) 
+@[simp] def Untyped.wk_composes {u: Untyped}: 
+  (σ ρ: Wk) -> (u.wk ρ).wk σ = u.wk (σ.comp ρ) 
   := by induction u <;> simp [*]
 
-theorem RawUntyped.wk_wk1 {u: RawUntyped}: u.wk RawWk.wk1 = u.wk1 
-  := rfl 
-
-@[simp] def Untyped.wk (u: Untyped m) (ρ: Wk n m): Untyped n :=
-  Untyped.mk (u.val.wk ρ.val) (RawUntyped.wk_bounds ρ.p u.p)
-
-@[simp] def Untyped.wk_composes {u: Untyped l} {σ: Wk n m} {ρ: Wk m l}:
-  (u.wk ρ).wk σ = u.wk (σ.comp ρ) := by simp
+theorem Untyped.wk_wk1 {u: Untyped}: u.wk Wk.wk1 = u.wk1 
+  := rfl
   
-theorem RawUntyped.step_wk1 {u: RawUntyped}: u.wk ρ.step = (u.wk ρ).wk1 
-  := by simp [<-RawWk.step_is_comp_wk1]
+theorem Untyped.step_wk1 {u: Untyped}: u.wk ρ.step = (u.wk ρ).wk1 
+  := by simp [<-Wk.step_is_comp_wk1]
 
-theorem RawUntyped.lift_wk1 {u: RawUntyped}: u.wk1.wk ρ.lift = (u.wk ρ).wk1 
+theorem Untyped.lift_wk1 {u: Untyped}: u.wk1.wk ρ.lift = (u.wk ρ).wk1 
   := by simp
